Ownership-Cut.dfy
@@ -1,4 +1,4 @@
-//imported from dafny/dahlia=-11.dfy
+          //imported from dafny/dahlia=-11.dfy
 
 include "Klon.dfy"
 include "Edges.dfy" //Edges
